Hacking.

theories/lifetime/definitions.v
@@ -3,6 +3,7 @@ From iris.prelude Require Export gmultiset strings.
 From iris.base_logic.lib Require Export invariants.
 From iris.base_logic.lib Require Import boxes.
 From iris.base_logic Require Import big_op.
+Import uPred.
 
 Definition lftN : namespace := nroot .@ "lft".
 Definition borN : namespace := lftN .@ "bor".
@@ -87,21 +88,21 @@ Section defs.
     | Bor_rebor κ' => ⌜κ ⊂ κ'⌝ ∗ own_cnt κ' (◯ 1)
     end%I.
 
-  Definition lft_bor_alive (κ : lft) (P : iProp Σ) : iProp Σ :=
+  Definition lft_bor_alive (κ : lft) (Pi : iProp Σ) : iProp Σ :=
     (∃ B : gmap slice_name bor_state,
-      box borN (bor_filled <$> B) P ∗
+      box borN (bor_filled <$> B) Pi ∗
       own_bor κ (● ((1%Qp,) ∘ DecAgree <$> B)) ∗
       [∗ map] s ∈ B, bor_cnt κ s)%I.
 
   Definition lft_bor_dead (κ : lft) : iProp Σ :=
-     (∃ (B: gset slice_name) (P : iProp Σ),
+     (∃ (B: gset slice_name) (Pb : iProp Σ),
        own_bor κ (● to_gmap (1%Qp, DecAgree Bor_in) B) ∗
-       box borN (to_gmap false B) P)%I.
+       box borN (to_gmap false B) Pb)%I.
 
-   Definition lft_inh (κ : lft) (s : bool) (P : iProp Σ) : iProp Σ :=
+   Definition lft_inh (κ : lft) (s : bool) (Pi : iProp Σ) : iProp Σ :=
      (∃ E : gset slice_name,
        own_inh κ (● GSet E) ∗
-       box inhN (to_gmap s E) P)%I.
+       box inhN (to_gmap s E) Pi)%I.
 
    Definition lft_vs_inv_go (κ : lft) (lft_inv_alive : ∀ κ', κ' ⊂ κ → iProp Σ)
        (I : gmap lft lft_names) : iProp Σ :=
@@ -110,33 +111,33 @@ Section defs.
        [∗ set] κ' ∈ dom _ I, ∀ Hκ : κ' ⊂ κ, lft_inv_alive κ' Hκ)%I.
 
    Definition lft_vs_go (κ : lft) (lft_inv_alive : ∀ κ', κ' ⊂ κ → iProp Σ)
-       (P Q : iProp Σ) : iProp Σ :=
+       (Pb Pi : iProp Σ) : iProp Σ :=
      (∃ n : nat,
        own_cnt κ (● n) ∗
        ∀ I : gmap lft lft_names,
-         lft_vs_inv_go κ lft_inv_alive I -∗ ▷ P -∗ lft_dead κ
+         lft_vs_inv_go κ lft_inv_alive I -∗ ▷ Pb -∗ lft_dead κ
            ={⊤∖↑mgmtN}=∗
-         lft_vs_inv_go κ lft_inv_alive I ∗ ▷ Q ∗ own_cnt κ (◯ n))%I.
+         lft_vs_inv_go κ lft_inv_alive I ∗ ▷ Pi ∗ own_cnt κ (◯ n))%I.
 
   Definition lft_inv_alive_go (κ : lft)
       (lft_inv_alive : ∀ κ', κ' ⊂ κ → iProp Σ) : iProp Σ :=
-    (∃ P Q,
-      lft_bor_alive κ P ∗
-      lft_vs_go κ lft_inv_alive P Q ∗
-      lft_inh κ false Q)%I.
+    (∃ Pb Pi,
+      lft_bor_alive κ Pb ∗
+      lft_vs_go κ lft_inv_alive Pb Pi ∗
+      lft_inh κ false Pi)%I.
 
   Definition lft_inv_alive (κ : lft) : iProp Σ :=
     Fix_F _ lft_inv_alive_go (gmultiset_wf κ).
   Definition lft_vs_inv (κ : lft) (I : gmap lft lft_names) : iProp Σ :=
     lft_vs_inv_go κ (λ κ' _, lft_inv_alive κ') I.
-  Definition lft_vs (κ : lft) (P Q : iProp Σ) : iProp Σ :=
-    lft_vs_go κ (λ κ' _, lft_inv_alive κ') P Q.
+  Definition lft_vs (κ : lft) (Pb Pi : iProp Σ) : iProp Σ :=
+    lft_vs_go κ (λ κ' _, lft_inv_alive κ') Pb Pi.
 
   Definition lft_inv_dead (κ : lft) : iProp Σ :=
-    (∃ P,
+    (∃ Pi,
       lft_bor_dead κ ∗
       own_cnt κ (● 0) ∗
-      lft_inh κ true P)%I.
+      lft_inh κ true Pi)%I.
 
   Definition lft_alive_in (A : gmap atomic_lft bool) (κ : lft) : Prop :=
     ∀ Λ:atomic_lft, Λ ∈ κ → A !! Λ = Some true.
@@ -193,3 +194,106 @@ Infix "⊑" := lft_incl (at level 70) : uPred_scope.
 Typeclasses Opaque lft_tok lft_dead bor_cnt lft_bor_alive lft_bor_dead
   lft_inh lft_inv_alive lft_vs_inv lft_vs lft_inv_dead lft_inv lft_incl
   idx_bor_own idx_bor raw_bor bor.
+
+Section basic_properties.
+Context `{invG Σ, lftG Σ}.
+Implicit Types κ : lft.
+
+(* Unfolding lemmas *)
+Lemma lft_vs_inv_go_ne κ (f f' : ∀ κ', κ' ⊂ κ → iProp Σ) I n :
+  (∀ κ' (Hκ : κ' ⊂ κ), f κ' Hκ ≡{n}≡ f' κ' Hκ) →
+  lft_vs_inv_go κ f I ≡{n}≡ lft_vs_inv_go κ f' I.
+Proof.
+  intros Hf. apply sep_ne, sep_ne, big_opS_ne=> // κ'.
+  by apply forall_ne=> Hκ.
+Qed.
+
+Lemma lft_vs_go_ne κ (f f' : ∀ κ', κ' ⊂ κ → iProp Σ) Pb Pb' Pi Pi' n :
+  (∀ κ' (Hκ : κ' ⊂ κ), f κ' Hκ ≡{n}≡ f' κ' Hκ) →
+  Pb ≡{n}≡ Pb' → Pi ≡{n}≡ Pi' →
+  lft_vs_go κ f Pb Pi ≡{n}≡ lft_vs_go κ f' Pb' Pi'.
+Proof.
+  intros Hf HPb HPi. apply exist_ne=> n'.
+  apply sep_ne, forall_ne=> // I. rewrite lft_vs_inv_go_ne //. solve_proper.
+Qed.
+
+Lemma lft_inv_alive_go_ne κ (f f' : ∀ κ', κ' ⊂ κ → iProp Σ) n :
+  (∀ κ' (Hκ : κ' ⊂ κ), f κ' Hκ ≡{n}≡ f' κ' Hκ) →
+  lft_inv_alive_go κ f ≡{n}≡ lft_inv_alive_go κ f'.
+Proof.
+  intros Hf. apply exist_ne=> Pb; apply exist_ne=> Pi. by rewrite lft_vs_go_ne.
+Qed.
+
+Lemma lft_inv_alive_unfold κ :
+  lft_inv_alive κ ⊣⊢ ∃ Pb Pi,
+    lft_bor_alive κ Pb ∗ lft_vs κ Pb Pi ∗ lft_inh κ false Pi.
+Proof.
+  apply equiv_dist=> n. rewrite /lft_inv_alive -Fix_F_eq.
+  apply lft_inv_alive_go_ne=> κ' Hκ.
+  apply (Fix_F_proper _ (λ _, dist n)); auto using lft_inv_alive_go_ne.
+Qed.
+Lemma lft_vs_inv_unfold κ (I : gmap lft lft_names) :
+  lft_vs_inv κ I ⊣⊢ lft_bor_dead κ ∗
+    own_ilft_auth I ∗
+    [∗ set] κ' ∈ dom _ I, ⌜κ' ⊂ κ⌝ → lft_inv_alive κ'.
+Proof.
+  rewrite /lft_vs_inv /lft_vs_inv_go. by setoid_rewrite pure_impl_forall.
+Qed.
+Lemma lft_vs_unfold κ Pb Pi :
+  lft_vs κ Pb Pi ⊣⊢ ∃ n : nat,
+    own_cnt κ (● n) ∗
+    ∀ I : gmap lft lft_names,
+      lft_vs_inv κ I -∗ ▷ Pb -∗ lft_dead κ ={⊤∖↑mgmtN}=∗
+      lft_vs_inv κ I ∗ ▷ Pi ∗ own_cnt κ (◯ n).
+Proof. done. Qed.
+
+Global Instance lft_bor_alive_ne κ n : Proper (dist n ==> dist n) (lft_bor_alive κ).
+Proof. solve_proper. Qed.
+Global Instance lft_bor_alive_proper κ : Proper ((≡) ==> (≡)) (lft_bor_alive κ).
+Proof. apply (ne_proper _). Qed.
+
+Global Instance lft_inh_ne κ s n : Proper (dist n ==> dist n) (lft_inh κ s).
+Proof. solve_proper. Qed.
+Global Instance lft_inh_proper κ s : Proper ((≡) ==> (≡)) (lft_inh κ s).
+Proof. apply (ne_proper _). Qed.
+
+Global Instance lft_vs_ne κ n :
+  Proper (dist n ==> dist n ==> dist n) (lft_vs κ).
+Proof. intros P P' HP Q Q' HQ. by apply lft_vs_go_ne. Qed.
+Global Instance lft_vs_proper κ : Proper ((≡) ==> (≡) ==> (≡)) (lft_vs κ).
+Proof. apply (ne_proper_2 _). Qed.
+
+Global Instance idx_bor_ne κ i n : Proper (dist n ==> dist n) (idx_bor κ i).
+Proof. solve_proper. Qed.
+Global Instance idx_bor_proper κ i : Proper ((≡) ==> (≡)) (idx_bor κ i).
+Proof. apply (ne_proper _). Qed.
+
+Global Instance raw_bor_ne i n : Proper (dist n ==> dist n) (raw_bor i).
+Proof. solve_proper. Qed.
+Global Instance raw_bor_proper i : Proper ((≡) ==> (≡)) (raw_bor i).
+Proof. apply (ne_proper _). Qed.
+
+Global Instance bor_ne κ n : Proper (dist n ==> dist n) (bor κ).
+Proof. solve_proper. Qed.
+Global Instance bor_proper κ : Proper ((≡) ==> (≡)) (bor κ).
+Proof. apply (ne_proper _). Qed.
+
+(*** PersistentP and TimelessP instances  *)
+Global Instance lft_tok_timeless q κ : TimelessP q.[κ].
+Proof. rewrite /lft_tok. apply _. Qed.
+Global Instance lft_dead_persistent κ : PersistentP [†κ].
+Proof. rewrite /lft_dead. apply _. Qed.
+Global Instance lft_dead_timeless κ : PersistentP [†κ].
+Proof. rewrite /lft_tok. apply _. Qed.
+
+Global Instance lft_incl_persistent κ κ' : PersistentP (κ ⊑ κ').
+Proof. rewrite /lft_incl. apply _. Qed.
+
+Global Instance idx_bor_persistent κ i P : PersistentP (&{κ,i} P).
+Proof. rewrite /idx_bor. apply _. Qed.
+Global Instance idx_borrow_own_timeless q i : TimelessP (idx_bor_own q i).
+Proof. rewrite /idx_bor_own. apply _. Qed.
+
+Global Instance lft_ctx_persistent : PersistentP lft_ctx.
+Proof. rewrite /lft_ctx. apply _. Qed.
+End basic_properties.
