theories/lifetime/primitive.v
@@ -8,167 +8,7 @@ Section primitive.
 Context `{invG Σ, lftG Σ}.
 Implicit Types κ : lft.
 
-(* Unfolding lemmas *)
-Lemma lft_vs_inv_go_ne κ (f f' : ∀ κ', κ' ⊂ κ → iProp Σ) I n :
-  (∀ κ' (Hκ : κ' ⊂ κ), f κ' Hκ ≡{n}≡ f' κ' Hκ) →
-  lft_vs_inv_go κ f I ≡{n}≡ lft_vs_inv_go κ f' I.
-Proof.
-  intros Hf. apply sep_ne, sep_ne, big_opS_ne=> // κ'.
-  by apply forall_ne=> Hκ.
-Qed.
-
-Lemma lft_vs_go_ne κ (f f' : ∀ κ', κ' ⊂ κ → iProp Σ) P P' Q Q' n :
-  (∀ κ' (Hκ : κ' ⊂ κ), f κ' Hκ ≡{n}≡ f' κ' Hκ) →
-  P ≡{n}≡ P' → Q ≡{n}≡ Q' →
-  lft_vs_go κ f P Q ≡{n}≡ lft_vs_go κ f' P' Q'.
-Proof.
-  intros Hf HP HQ. apply exist_ne=> n'.
-  apply sep_ne, forall_ne=> // I. rewrite lft_vs_inv_go_ne //. solve_proper.
-Qed.
-
-Lemma lft_inv_alive_go_ne κ (f f' : ∀ κ', κ' ⊂ κ → iProp Σ) n :
-  (∀ κ' (Hκ : κ' ⊂ κ), f κ' Hκ ≡{n}≡ f' κ' Hκ) →
-  lft_inv_alive_go κ f ≡{n}≡ lft_inv_alive_go κ f'.
-Proof.
-  intros Hf. apply exist_ne=> P; apply exist_ne=> Q. by rewrite lft_vs_go_ne.
-Qed.
-
-Lemma lft_inv_alive_unfold κ :
-  lft_inv_alive κ ⊣⊢ ∃ P Q, lft_bor_alive κ P ∗ lft_vs κ P Q ∗ lft_inh κ false Q.
-Proof.
-  apply equiv_dist=> n. rewrite /lft_inv_alive -Fix_F_eq.
-  apply lft_inv_alive_go_ne=> κ' Hκ.
-  apply (Fix_F_proper _ (λ _, dist n)); auto using lft_inv_alive_go_ne.
-Qed.
-Lemma lft_vs_inv_unfold κ (I : gmap lft lft_names) :
-  lft_vs_inv κ I ⊣⊢ lft_bor_dead κ ∗
-    own_ilft_auth I ∗
-    [∗ set] κ' ∈ dom _ I, ⌜κ' ⊂ κ⌝ → lft_inv_alive κ'.
-Proof.
-  rewrite /lft_vs_inv /lft_vs_inv_go. by setoid_rewrite pure_impl_forall.
-Qed.
-Lemma lft_vs_unfold κ P Q :
-  lft_vs κ P Q ⊣⊢ ∃ n : nat,
-    own_cnt κ (● n) ∗
-    ∀ I : gmap lft lft_names,
-      lft_vs_inv κ I -∗ ▷ P -∗ lft_dead κ ={⊤∖↑mgmtN}=∗
-      lft_vs_inv κ I ∗ ▷ Q ∗ own_cnt κ (◯ n).
-Proof. done. Qed.
-
-Global Instance lft_bor_alive_ne κ n : Proper (dist n ==> dist n) (lft_bor_alive κ).
-Proof. solve_proper. Qed.
-Global Instance lft_bor_alive_proper κ : Proper ((≡) ==> (≡)) (lft_bor_alive κ).
-Proof. apply (ne_proper _). Qed.
-
-Global Instance lft_inh_ne κ s n : Proper (dist n ==> dist n) (lft_inh κ s).
-Proof. solve_proper. Qed.
-Global Instance lft_inh_proper κ s : Proper ((≡) ==> (≡)) (lft_inh κ s).
-Proof. apply (ne_proper _). Qed.
-
-Global Instance lft_vs_ne κ n :
-  Proper (dist n ==> dist n ==> dist n) (lft_vs κ).
-Proof. intros P P' HP Q Q' HQ. by apply lft_vs_go_ne. Qed.
-Global Instance lft_vs_proper κ : Proper ((≡) ==> (≡) ==> (≡)) (lft_vs κ).
-Proof. apply (ne_proper_2 _). Qed.
-
-Global Instance idx_bor_ne κ i n : Proper (dist n ==> dist n) (idx_bor κ i).
-Proof. solve_proper. Qed.
-Global Instance idx_bor_proper κ i : Proper ((≡) ==> (≡)) (idx_bor κ i).
-Proof. apply (ne_proper _). Qed.
-
-Global Instance raw_bor_ne i n : Proper (dist n ==> dist n) (raw_bor i).
-Proof. solve_proper. Qed.
-Global Instance raw_bor_proper i : Proper ((≡) ==> (≡)) (raw_bor i).
-Proof. apply (ne_proper _). Qed.
-
-Global Instance bor_ne κ n : Proper (dist n ==> dist n) (bor κ).
-Proof. solve_proper. Qed.
-Global Instance bor_proper κ : Proper ((≡) ==> (≡)) (bor κ).
-Proof. apply (ne_proper _). Qed.
-
-(*** PersistentP and TimelessP instances  *)
-Global Instance lft_tok_timeless q κ : TimelessP q.[κ].
-Proof. rewrite /lft_tok. apply _. Qed.
-Global Instance lft_dead_persistent κ : PersistentP [†κ].
-Proof. rewrite /lft_dead. apply _. Qed.
-Global Instance lft_dead_timeless κ : PersistentP [†κ].
-Proof. rewrite /lft_tok. apply _. Qed.
-
-Global Instance lft_incl_persistent κ κ' : PersistentP (κ ⊑ κ').
-Proof. rewrite /lft_incl. apply _. Qed.
-
-Global Instance idx_bor_persistent κ i P : PersistentP (&{κ,i} P).
-Proof. rewrite /idx_bor. apply _. Qed.
-Global Instance idx_borrow_own_timeless q i : TimelessP (idx_bor_own q i).
-Proof. rewrite /idx_bor_own. apply _. Qed.
-
-Global Instance lft_ctx_persistent : PersistentP lft_ctx.
-Proof. rewrite /lft_ctx. apply _. Qed.
-
-(** Alive and dead *)
-Global Instance lft_alive_in_dec A κ : Decision (lft_alive_in A κ).
-Proof.
-  refine (cast_if (decide (set_Forall (λ Λ, A !! Λ = Some true)
-                  (dom (gset atomic_lft) κ))));
-    rewrite /lft_alive_in; by setoid_rewrite <-gmultiset_elem_of_dom.
-Qed.
-Global Instance lft_dead_in_dec A κ : Decision (lft_dead_in A κ).
-Proof.
-  refine (cast_if (decide (set_Exists (λ Λ, A !! Λ = Some false)
-                  (dom (gset atomic_lft) κ))));
-      rewrite /lft_dead_in; by setoid_rewrite <-gmultiset_elem_of_dom.
-Qed.
-
-Lemma lft_alive_or_dead_in A κ :
-  (∃ Λ, Λ ∈ κ ∧ A !! Λ = None) ∨ (lft_alive_in A κ ∨ lft_dead_in A κ).
-Proof.
-  rewrite /lft_alive_in /lft_dead_in.
-  destruct (decide (set_Exists (λ Λ, A !! Λ = None) (dom (gset _) κ)))
-    as [(Λ & ?%gmultiset_elem_of_dom & HAΛ)|HA%(not_set_Exists_Forall _)]; first eauto.
-  destruct (decide (set_Exists (λ Λ, A !! Λ = Some false) (dom (gset _) κ)))
-    as [(Λ & HΛ%gmultiset_elem_of_dom & ?)|HA'%(not_set_Exists_Forall _)]; first eauto.
-  right; left. intros Λ HΛ%gmultiset_elem_of_dom.
-  move: (HA _ HΛ) (HA' _ HΛ)=> /=. case: (A !! Λ)=>[[]|]; naive_solver.
-Qed.
-Lemma lft_alive_and_dead_in A κ : lft_alive_in A κ → lft_dead_in A κ → False.
-Proof. intros Halive (Λ&HΛ&?). generalize (Halive _ HΛ). naive_solver. Qed.
-
-Lemma lft_alive_in_subseteq A κ κ' :
-  lft_alive_in A κ → κ' ⊆ κ → lft_alive_in A κ'.
-Proof. intros Halive ? Λ ?. by eapply Halive, gmultiset_elem_of_subseteq. Qed.
-
-Lemma lft_alive_in_insert A κ Λ b :
-  A !! Λ = None → lft_alive_in A κ → lft_alive_in (<[Λ:=b]> A) κ.
-Proof.
-  intros HΛ Halive Λ' HΛ'.
-  assert (Λ ≠ Λ') by (intros ->; move:(Halive _ HΛ'); by rewrite HΛ).
-  rewrite lookup_insert_ne; eauto.
-Qed.
-Lemma lft_alive_in_insert_false A κ Λ b :
-  Λ ∉ κ → lft_alive_in A κ → lft_alive_in (<[Λ:=b]> A) κ.
-Proof.
-  intros HΛ Halive Λ' HΛ'.
-  rewrite lookup_insert_ne; last (by intros ->); auto.
-Qed.
-
-Lemma lft_dead_in_insert A κ Λ b :
-  A !! Λ = None → lft_dead_in A κ → lft_dead_in (<[Λ:=b]> A) κ.
-Proof.
-  intros HΛ (Λ'&?&HΛ').
-  assert (Λ ≠ Λ') by (intros ->; move:HΛ'; by rewrite HΛ).
-  exists Λ'. by rewrite lookup_insert_ne.
-Qed.
-Lemma lft_dead_in_insert_false A κ Λ :
-  lft_dead_in A κ → lft_dead_in (<[Λ:=false]> A) κ.
-Proof.
-  intros (Λ'&?&HΛ'). destruct (decide (Λ = Λ')) as [<-|].
-  - exists Λ. by rewrite lookup_insert.
-  - exists Λ'. by rewrite lookup_insert_ne.
-Qed.
-Lemma lft_dead_in_insert_false' A κ Λ : Λ ∈ κ → lft_dead_in (<[Λ:=false]> A) κ.
-Proof. exists Λ. by rewrite lookup_insert. Qed.
-
-(** Silly stuff *)
+(** Ownership *)
 Lemma own_ilft_auth_agree (I : gmap lft lft_names) κ γs :
   own_ilft_auth I ⊢
     own ilft_name (◯ {[κ := DecAgree γs]}) -∗ ⌜is_Some (I !! κ)⌝.
@@ -267,12 +107,86 @@ Proof.
   iDestruct 1 as (γs) "[#Hκ Hx]"; iExists γs. iFrame "Hκ". by iApply own_update.
 Qed.
 
+(** Alive and dead *)
+Global Instance lft_alive_in_dec A κ : Decision (lft_alive_in A κ).
+Proof.
+  refine (cast_if (decide (set_Forall (λ Λ, A !! Λ = Some true)
+                  (dom (gset atomic_lft) κ))));
+    rewrite /lft_alive_in; by setoid_rewrite <-gmultiset_elem_of_dom.
+Qed.
+Global Instance lft_dead_in_dec A κ : Decision (lft_dead_in A κ).
+Proof.
+  refine (cast_if (decide (set_Exists (λ Λ, A !! Λ = Some false)
+                  (dom (gset atomic_lft) κ))));
+      rewrite /lft_dead_in; by setoid_rewrite <-gmultiset_elem_of_dom.
+Qed.
+
+Lemma lft_alive_or_dead_in A κ :
+  (∃ Λ, Λ ∈ κ ∧ A !! Λ = None) ∨ (lft_alive_in A κ ∨ lft_dead_in A κ).
+Proof.
+  rewrite /lft_alive_in /lft_dead_in.
+  destruct (decide (set_Exists (λ Λ, A !! Λ = None) (dom (gset _) κ)))
+    as [(Λ & ?%gmultiset_elem_of_dom & HAΛ)|HA%(not_set_Exists_Forall _)]; first eauto.
+  destruct (decide (set_Exists (λ Λ, A !! Λ = Some false) (dom (gset _) κ)))
+    as [(Λ & HΛ%gmultiset_elem_of_dom & ?)|HA'%(not_set_Exists_Forall _)]; first eauto.
+  right; left. intros Λ HΛ%gmultiset_elem_of_dom.
+  move: (HA _ HΛ) (HA' _ HΛ)=> /=. case: (A !! Λ)=>[[]|]; naive_solver.
+Qed.
+Lemma lft_alive_and_dead_in A κ : lft_alive_in A κ → lft_dead_in A κ → False.
+Proof. intros Halive (Λ&HΛ&?). generalize (Halive _ HΛ). naive_solver. Qed.
+
+Lemma lft_alive_in_subseteq A κ κ' :
+  lft_alive_in A κ → κ' ⊆ κ → lft_alive_in A κ'.
+Proof. intros Halive ? Λ ?. by eapply Halive, gmultiset_elem_of_subseteq. Qed.
+
+Lemma lft_alive_in_insert A κ Λ b :
+  A !! Λ = None → lft_alive_in A κ → lft_alive_in (<[Λ:=b]> A) κ.
+Proof.
+  intros HΛ Halive Λ' HΛ'.
+  assert (Λ ≠ Λ') by (intros ->; move:(Halive _ HΛ'); by rewrite HΛ).
+  rewrite lookup_insert_ne; eauto.
+Qed.
+Lemma lft_alive_in_insert_false A κ Λ b :
+  Λ ∉ κ → lft_alive_in A κ → lft_alive_in (<[Λ:=b]> A) κ.
+Proof.
+  intros HΛ Halive Λ' HΛ'.
+  rewrite lookup_insert_ne; last (by intros ->); auto.
+Qed.
+
+Lemma lft_dead_in_insert A κ Λ b :
+  A !! Λ = None → lft_dead_in A κ → lft_dead_in (<[Λ:=b]> A) κ.
+Proof.
+  intros HΛ (Λ'&?&HΛ').
+  assert (Λ ≠ Λ') by (intros ->; move:HΛ'; by rewrite HΛ).
+  exists Λ'. by rewrite lookup_insert_ne.
+Qed.
+Lemma lft_dead_in_insert_false A κ Λ :
+  lft_dead_in A κ → lft_dead_in (<[Λ:=false]> A) κ.
+Proof.
+  intros (Λ'&?&HΛ'). destruct (decide (Λ = Λ')) as [<-|].
+  - exists Λ. by rewrite lookup_insert.
+  - exists Λ'. by rewrite lookup_insert_ne.
+Qed.
+Lemma lft_dead_in_insert_false' A κ Λ : Λ ∈ κ → lft_dead_in (<[Λ:=false]> A) κ.
+Proof. exists Λ. by rewrite lookup_insert. Qed.
+
 Lemma lft_inv_alive_twice κ : lft_inv_alive κ ⊢ lft_inv_alive κ -∗ False.
 Proof.
   rewrite lft_inv_alive_unfold /lft_inh.
   iDestruct 1 as (P Q) "(_&_&Hinh)"; iDestruct 1 as (P' Q') "(_&_&Hinh')".
   iDestruct "Hinh" as (E) "[HE _]"; iDestruct "Hinh'" as (E') "[HE' _]".
   by iDestruct (own_inh_valid_2 with "HE HE'") as %?.
+Qed.
+
+Lemma lft_inv_alive_in A κ : lft_alive_in A κ → lft_inv A κ -∗ lft_inv_alive κ.
+Proof.
+  rewrite /lft_inv. iIntros (?) "[[$ _]|[_ %]]".
+  by destruct (lft_alive_and_dead_in A κ).
+Qed.
+Lemma lft_inv_dead_in A κ : lft_dead_in A κ → lft_inv A κ -∗ lft_inv_dead κ.
+Proof.
+  rewrite /lft_inv. iIntros (?) "[[_ %]|[$ _]]".
+  by destruct (lft_alive_and_dead_in A κ).
 Qed.
 
 (** Basic rules about lifetimes  *)
